src/kemedhoc/Impl.KEMEDHOC.Parser.fst
@@ -1,0 +1,110 @@
+module Impl.KEMEDHOC.Parser
+
+(*LowStar related modules*)
+module B = LowStar.Buffer
+module ST = FStar.HyperStack.ST
+module HS = FStar.HyperStack
+module S = FStar.Seq
+module Seq = Lib.Sequence
+
+module Spec = Spec.KEMEDHOC.Parser
+friend Spec.KEMEDHOC.Parser
+
+module SpecCrypto = Spec.KEMEDHOC.CryptoPrimitives
+
+open Impl.EDHOC.Utilities
+
+(*--------------------------------------*)
+(*---------------------------- Parsing*)
+(*--------------------------------------*)
+
+/// ------------------------
+/// Plaintext 1
+/// ------------------------
+let concat_ptx1 p1 p1_buffer
+    = concat_buff2 p1.id_cred_I p1.cred_I p1_buffer
+
+let deserialize_ptx1 p1_buffer p1
+    = (**) let h0 = ST.get () in
+    let id_cred_I_buffer = sub p1_buffer 0ul (size Spec.id_cred_size) in
+    copy p1.id_cred_I id_cred_I_buffer;
+    (**) let h1 = ST.get () in
+    (**) assert(modifies1 (p1.id_cred_I) h0 h1);
+    
+    let cred_I_buffer = sub p1_buffer (size Spec.id_cred_size) (size Spec.cred_size) in
+    copy p1.cred_I cred_I_buffer;
+    (**) let h2 = ST.get () in
+    assert(modifies2 p1.id_cred_I p1.cred_I h0 h2);
+    ()
+
+/// ------------------------
+/// Message 1
+/// ------------------------
+let concat_msg1 kcs msg1 msg1_buffer
+    = concat_buff6 msg1.method msg1.suite_i msg1.pk_x msg1.ct_auth_R msg1.c_i msg1.c1 msg1_buffer
+
+/// ------------------------
+/// Plaintext 2
+/// ------------------------
+let concat_ptx2 kcs p2 p2_buffer
+    = concat_buff4 p2.c_R p2.id_cred_R p2.cred_R p2.mac2 p2_buffer
+
+let deserialize_ptx2 kcs p2_buffer p2
+    = (**) let h0 = ST.get () in
+    let c_R_buffer = sub p2_buffer 0ul (size Spec.c_id_size) in
+    copy p2.c_R c_R_buffer;
+    (**) let h1 = ST.get () in
+    (**) assert(modifies1 (p2.c_R) h0 h1);
+    
+    let id_cred_R_buffer = sub p2_buffer (size Spec.c_id_size) (size Spec.id_cred_size) in
+    copy p2.id_cred_R id_cred_R_buffer;
+    (**) let h2 = ST.get () in
+    assert(modifies2 p2.c_R p2.id_cred_R h0 h2);
+    
+    let cred_R_buffer = sub p2_buffer (size Spec.c_id_size +! size Spec.id_cred_size) (size Spec.cred_size) in
+    copy p2.cred_R cred_R_buffer;
+    (**) let h3 = ST.get () in
+    assert(modifies3 p2.c_R p2.id_cred_R p2.cred_R h0 h3);
+    
+    let mac2_buffer = sub p2_buffer (size Spec.c_id_size +! size Spec.id_cred_size +! size Spec.cred_size) (size (SpecCrypto.mac23_size kcs)) in
+    copy p2.mac2 mac2_buffer;
+    (**) let h4 = ST.get () in
+    assert(modifies4 p2.c_R p2.id_cred_R p2.cred_R p2.mac2 h0 h4);
+    ()
+
+/// ------------------------
+/// Message 2
+/// ------------------------
+let concat_msg2 kcs msg2 msg2_buffer
+    = concat_buff3 msg2.ct_y msg2.ct_auth_I msg2.c2 msg2_buffer
+
+/// ------------------------
+/// Plaintext 3
+/// ------------------------
+let concat_ptx3 kcs p3 p3_buffer
+    = concat_buff2 p3.id_cred_I p3.mac3 p3_buffer
+
+let deserialize_ptx3 kcs p3_buffer p3
+    = (**) let h0 = ST.get () in
+    let id_cred_I_buffer = sub p3_buffer 0ul (size Spec.id_cred_size) in
+    copy p3.id_cred_I id_cred_I_buffer;
+    (**) let h1 = ST.get () in
+    (**) assert(modifies1 (p3.id_cred_I) h0 h1);
+    (**) assert(
+        let p3_s = Spec.deserialize_ptx3 #kcs (as_seq h0 p3_buffer) in
+        Seq.equal p3_s.id_cred_I (as_seq h1 p3.id_cred_I)
+    );
+
+    let mac3_buffer = sub p3_buffer (size Spec.id_cred_size) (size (SpecCrypto.mac23_size kcs)) in
+    copy p3.mac3 mac3_buffer;
+    (**) let h2 = ST.get () in
+    (**) assert(modifies1 p3.mac3 h1 h2);
+    (**) assert(modifies2 p3.id_cred_I p3.mac3 h0 h2);
+    (**) assert(
+        let p3_s = Spec.deserialize_ptx3 #kcs (as_seq h0 p3_buffer) in
+        let p3_s_deserd = plaintext3_eval h2 p3 in
+
+        Seq.equal p3_s.mac3 (as_seq h2 p3.mac3)
+        /\ Seq.equal p3_s.mac3 p3_s_deserd.mac3
+    );
+    ()
