src/kemedhoc/Impl.KEMEDHOC.Parser.fsti
@@ -1,0 +1,410 @@
+module Impl.KEMEDHOC.Parser
+
+(*HACL related modules*)
+// open Lib.RawIntTypes
+open Lib.IntTypes
+// open Lib.Sequence
+open Lib.ByteBuffer
+// lbuffer type, an immutable buffer with
+// length tag, is from this module
+// let lbuffer (a:Type0) (len:size_t) = lbuffer_t MUT a len
+// `live` and `disjoint` are also from this module.
+// Basically, HACL `Lib.Buffer` is a wrapper of `LowStar.Buffer`
+// and related LowStar memory models.
+open Lib.Buffer
+
+open Impl.KEMEDHOC.Types
+
+(*LowStar related modules*)
+module B = LowStar.Buffer
+module ST = FStar.HyperStack.ST
+module HS = FStar.HyperStack
+module S = FStar.Seq
+module Seq = Lib.Sequence
+
+open Spec.KEMEDHOC.Base.Definitions
+module Spec = Spec.KEMEDHOC.Parser
+module SpecCrypto = Spec.KEMEDHOC.CryptoPrimitives
+module SpecSerdEdhoc = Spec.EDHOC.Serialization
+
+open LowStar.BufferOps
+
+open Impl.KEMEDHOC.CryptoPrimitives
+
+
+(*---------------------------- Utility buffers*)
+inline_for_extraction
+type c_id_buffer = lbuffer uint8 (size Spec.c_id_size)
+inline_for_extraction
+type id_cred_buffer = lbuffer uint8 (size Spec.id_cred_size)
+inline_for_extraction
+type cred_buffer = lbuffer uint8 (size Spec.cred_size)
+
+(*---------------------------- Plaintext 1*)
+unopteq type plaintext1 = {
+    id_cred_I: id_cred_buffer;
+    cred_I: cred_buffer
+}
+
+let plaintext1_disjoint (p1: plaintext1)
+    = disjoint p1.id_cred_I p1.cred_I
+
+let plaintext1_live (h: HS.mem) (p1: plaintext1) 
+    = live h p1.id_cred_I /\ live h p1.cred_I
+
+let is_valid_plaintext1 (h: HS.mem) (p1: plaintext1)
+    = plaintext1_disjoint p1 /\ plaintext1_live h p1
+
+let plaintext1_union (p1: plaintext1)
+    = loc p1.id_cred_I |+| loc p1.cred_I
+
+let plaintext1_modifies (p1: plaintext1) (h0 h1: HS.mem)
+    = modifies (plaintext1_union p1) h0 h1
+
+let lemma_plaintext1_union_disjoint (#len: size_t) (h: HS.mem) (p1: plaintext1) (b: lbuffer uint8 len)
+    : Lemma (requires is_valid_plaintext1 h p1)
+    (ensures B.loc_disjoint (loc b) (plaintext1_union p1) <==> B.all_disjoint [loc b; loc p1.id_cred_I; loc p1.cred_I])
+    = ()
+
+// convert the low-level plaintext1 to the high-level sequence
+let plaintext1_eval (h: HS.mem) (p1: plaintext1)
+    : GTot (Spec.plaintext1)
+    = {
+        id_cred_I = as_seq h p1.id_cred_I;
+        cred_I = as_seq h p1.cred_I
+    }
+
+(*---------------------------- Message 1 Type*)
+unopteq type message1 (kcs: supportedKemCipherSuite) = {
+    method: lbuffer uint8 1ul; // 1 byte
+    suite_i: lbuffer uint8 1ul; // 1 byte
+    pk_x: kem_pub_key_buff kcs;
+    ct_auth_R: kem_ciphertext_buff kcs;
+    c_i: c_id_buffer;
+    c1: c1_buff kcs;
+    // does not support EAD1
+}
+
+let message1_disjoint (#kcs: supportedKemCipherSuite) (m1: message1 kcs)
+    = B.all_disjoint [loc m1.method; loc m1.suite_i; loc m1.pk_x; loc m1.ct_auth_R; loc m1.c_i; loc m1.c1]
+
+let message1_live (#kcs: supportedKemCipherSuite) (h: HS.mem) (m1: message1 kcs)
+    = live h m1.method /\ live h m1.suite_i /\live h m1.pk_x
+    /\ live h m1.ct_auth_R /\ live h m1.c_i /\ live h m1.c1
+
+let is_legit_message1 (#kcs: supportedKemCipherSuite) (h: HS.mem) (m1: message1 kcs) 
+    = (SpecSerdEdhoc.bytes_to_nat (as_seq h m1.method) = 5)
+      /\ (SpecSerdEdhoc.bytes_to_nat (as_seq h m1.suite_i) = 9)
+
+let is_valid_message1 (#kcs: supportedKemCipherSuite) (h: HS.mem) (m1: message1 kcs) 
+    = message1_disjoint m1 /\ message1_live h m1
+    /\ is_legit_message1 h m1
+      
+
+type legitMessage1 (kcs: supportedKemCipherSuite) (h: HS.mem) = m1:message1 kcs{is_legit_message1 h m1} 
+
+// convert the low-level message1 to the high-level sequence
+let message1_eval (#kcs: supportedKemCipherSuite) (h: HS.mem) (m1: legitMessage1 kcs h) 
+    : GTot (Spec.message1 #kcs)
+    = let method_nat = SpecSerdEdhoc.bytes_to_nat (as_seq h m1.method) in
+    let suite_label = SpecSerdEdhoc.bytes_to_nat (as_seq h m1.suite_i) in
+    {
+        method = nat_to_method method_nat;
+        suite_i = suite_label;
+        pk_x = as_seq h m1.pk_x;
+        ct_auth_R = as_seq h m1.ct_auth_R;
+        c_i = as_seq h m1.c_i;
+        c1 = as_seq h m1.c1
+    }
+
+let message1_union (#kcs: supportedKemCipherSuite) (m1: message1 kcs)
+    = loc m1.method |+| loc m1.suite_i |+| loc m1.pk_x
+    |+| loc m1.ct_auth_R |+| loc m1.c_i |+| loc m1.c1
+
+(*---------------------------- Plaintext 2*)
+unopteq type plaintext2 (kcs: supportedKemCipherSuite) = {
+    c_R: c_id_buffer;
+    id_cred_R: id_cred_buffer;
+    cred_R: cred_buffer;
+    // does not support EAD2
+    mac2: mac23_buff kcs;
+}
+
+let plaintext2_disjoint (#kcs: supportedKemCipherSuite) (p2: plaintext2 kcs)
+    = B.all_disjoint [loc p2.c_R; loc p2.id_cred_R; loc p2.cred_R; loc p2.mac2]
+
+let plaintext2_live (#kcs: supportedKemCipherSuite) (h: HS.mem) (p2: plaintext2 kcs)
+    = live h p2.c_R /\ live h p2.id_cred_R /\ live h p2.cred_R /\ live h p2.mac2
+
+let is_valid_plaintext2 (#kcs: supportedKemCipherSuite) (h: HS.mem) (p2: plaintext2 kcs)
+    = plaintext2_disjoint p2 /\ plaintext2_live h p2
+
+let plaintext2_union (#kcs: supportedKemCipherSuite) (p2: plaintext2 kcs)
+    = loc p2.c_R |+| loc p2.id_cred_R |+| loc p2.cred_R |+| loc p2.mac2
+
+// convert the low-level plaintext2 to the high-level sequence
+let plaintext2_eval (#kcs: supportedKemCipherSuite) (h: HS.mem) (p2: plaintext2 kcs)
+    : GTot (Spec.plaintext2 #kcs)
+    = {
+        c_R = as_seq h p2.c_R;
+        id_cred_R = as_seq h p2.id_cred_R;
+        cred_R = as_seq h p2.cred_R;
+        mac2 = as_seq h p2.mac2
+    }
+
+let plaintext2_modifies (#kcs: supportedKemCipherSuite) (p2: plaintext2 kcs) (h0 h1: HS.mem)
+    = modifies (plaintext2_union p2) h0 h1
+
+(*---------------------------- Message 2 Type*)
+unopteq type message2 (kcs: supportedKemCipherSuite) = {
+    ct_y: kem_ciphertext_buff kcs;
+    ct_auth_I: kem_ciphertext_buff kcs;
+    c2: c2_buff kcs;
+    // does not support EAD2
+}
+
+let message2_disjoint (#kcs: supportedKemCipherSuite) (m2: message2 kcs)
+    = B.all_disjoint [loc m2.ct_y; loc m2.ct_auth_I; loc m2.c2]
+
+let message2_live (#kcs: supportedKemCipherSuite) (h: HS.mem) (m2: message2 kcs)
+    = live h m2.ct_y /\ live h m2.ct_auth_I /\ live h m2.c2
+
+let is_valid_message2 (#kcs: supportedKemCipherSuite) (h: HS.mem) (m2: message2 kcs)
+    = message2_disjoint m2 /\ message2_live h m2
+
+let message2_union (#kcs: supportedKemCipherSuite) (m2: message2 kcs)
+    = loc m2.ct_y |+| loc m2.ct_auth_I |+| loc m2.c2
+
+// convert the low-level message2 to the high-level sequence
+let message2_eval (#kcs: supportedKemCipherSuite) (h: HS.mem) (m2: message2 kcs)
+    : GTot (Spec.message2 #kcs)
+    = {
+        ct_y = as_seq h m2.ct_y;
+        ct_auth_I = as_seq h m2.ct_auth_I;
+        c2 = as_seq h m2.c2
+    }
+
+(*---------------------------- Plaintext 3*)
+unopteq type plaintext3 (kcs: supportedKemCipherSuite) = {
+    id_cred_I: id_cred_buffer;
+    // does not support EAD3
+    mac3: mac23_buff kcs
+}
+
+let plaintext3_disjoint (#kcs: supportedKemCipherSuite) (p3: plaintext3 kcs)
+    = disjoint p3.id_cred_I p3.mac3
+
+let plaintext3_live (#kcs: supportedKemCipherSuite) (h: HS.mem) (p3: plaintext3 kcs)
+    = live h p3.id_cred_I /\ live h p3.mac3
+
+let is_valid_plaintext3 (#kcs: supportedKemCipherSuite) (h: HS.mem) (p3: plaintext3 kcs)
+    = plaintext3_disjoint p3 /\ plaintext3_live h p3
+
+let plaintext3_union (#kcs: supportedKemCipherSuite) (p3: plaintext3 kcs)
+    = loc p3.id_cred_I |+| loc p3.mac3
+
+// convert the low-level plaintext3 to the high-level sequence
+let plaintext3_eval (#kcs: supportedKemCipherSuite) (h: HS.mem) (p3: plaintext3 kcs)
+    : GTot (Spec.plaintext3 #kcs)
+    = {
+        id_cred_I = as_seq h p3.id_cred_I;
+        mac3 = as_seq h p3.mac3
+    }
+
+let plaintext3_modifies (#kcs: supportedKemCipherSuite) (p3: plaintext3 kcs) (h0 h1: HS.mem)
+    = modifies (plaintext3_union p3) h0 h1
+
+(*---------------------------- Message 3 Type*)
+type message3 (kcs: supportedKemCipherSuite) = lbuffer uint8 (size (Spec.c3_size kcs))
+
+(*--------------------------------------*)
+(*---------------------------- Parsing*)
+(*--------------------------------------*)
+
+/// ------------------------
+/// Plaintext 1
+/// ------------------------
+let construct_plaintext1 (id_cred_I: id_cred_buffer)
+    (cred_I: cred_buffer)
+    : Tot plaintext1
+    = { id_cred_I = id_cred_I; cred_I = cred_I }
+
+val concat_ptx1:
+    p1: plaintext1
+    -> p1_buffer: plaintext1_buff
+    -> ST.Stack unit
+    (requires fun h0 ->
+        is_valid_plaintext1 h0 p1
+        /\ live h0 p1_buffer
+        /\ B.loc_disjoint (loc p1_buffer) (plaintext1_union p1)
+    )
+    (ensures fun h0 _ h1 ->
+        let p1_s = plaintext1_eval h0 p1 in
+        let p1_s_concat = Spec.concat_ptx1 p1_s in
+
+        modifies1 p1_buffer h0 h1
+        /\ Seq.equal (as_seq h1 p1_buffer) p1_s_concat
+    )
+
+val deserialize_ptx1:
+    p1_buffer: plaintext1_buff
+    -> p1: plaintext1
+    -> ST.Stack unit
+    (requires fun h0 ->
+        live h0 p1_buffer /\ is_valid_plaintext1 h0 p1
+        /\ B.loc_disjoint (loc p1_buffer) (plaintext1_union p1)
+    )
+    (ensures fun h0 _ h1 ->
+        let p1_s_deserd = plaintext1_eval h1 p1 in
+        let p1_s = Spec.deserialize_ptx1 (as_seq h0 p1_buffer) in
+
+        plaintext1_modifies p1 h0 h1
+        /\ Seq.equal p1_s_deserd.id_cred_I p1_s.id_cred_I
+        /\ Seq.equal p1_s_deserd.cred_I p1_s.cred_I
+    )
+
+/// ------------------------
+/// Message 1
+/// ------------------------
+let construct_message1 (kcs: supportedKemCipherSuite)
+    (method: lbuffer uint8 1ul) (suite_i: lbuffer uint8 1ul)
+    (pk_x: kem_pub_key_buff kcs) (ct_auth_R: kem_ciphertext_buff kcs)
+    (c_i: c_id_buffer) (c1: c1_buff kcs)
+    : Tot (message1 kcs)
+    = { method = method; suite_i = suite_i; pk_x = pk_x; ct_auth_R = ct_auth_R; c_i = c_i; c1 = c1 }
+
+val concat_msg1:
+    kcs: supportedKemCipherSuite
+    -> msg1: message1 kcs
+    -> msg1_buffer: lbuffer uint8 (size (Spec.concat_msg1_fixed_length kcs))
+    -> ST.Stack unit
+    (requires fun h0 ->
+        is_valid_message1 h0 msg1 /\ live h0 msg1_buffer
+        /\ B.loc_disjoint (loc msg1_buffer) (message1_union msg1)
+    )
+    (ensures fun h0 _ h1 ->
+        let m1_s = message1_eval h0 msg1 in
+        let m1_s_concat = Spec.concat_msg1 #kcs m1_s in
+
+        modifies1 msg1_buffer h0 h1
+        /\ Seq.equal (as_seq h1 msg1_buffer) m1_s_concat
+    )
+
+/// ------------------------
+/// Plaintext 2
+/// ------------------------
+let construct_plaintext2 (kcs: supportedKemCipherSuite)
+    (c_R: c_id_buffer) (id_cred_R: id_cred_buffer)
+    (cred_R: cred_buffer) (mac2: mac23_buff kcs)
+    : Tot (plaintext2 kcs)
+    = { c_R = c_R; id_cred_R = id_cred_R; cred_R = cred_R; mac2 = mac2 }
+
+val concat_ptx2:
+    kcs: supportedKemCipherSuite
+    -> p2: plaintext2 kcs
+    -> p2_buffer: plaintext2_buff kcs
+    -> ST.Stack unit
+    (requires fun h0 ->
+        is_valid_plaintext2 h0 p2 /\ live h0 p2_buffer
+        /\ B.loc_disjoint (loc p2_buffer) (plaintext2_union p2)
+    )
+    (ensures fun h0 _ h1 ->
+        let p2_s = plaintext2_eval #kcs h0 p2 in
+        let p2_s_concat = Spec.concat_ptx2 #kcs p2_s in
+
+        modifies1 p2_buffer h0 h1
+        /\ Seq.equal (as_seq h1 p2_buffer) p2_s_concat
+    )
+
+val deserialize_ptx2:
+    kcs: supportedKemCipherSuite
+    -> p2_buffer: plaintext2_buff kcs
+    -> p2: plaintext2 kcs
+    -> ST.Stack unit
+    (requires fun h0 ->
+        is_valid_plaintext2 h0 p2 /\ live h0 p2_buffer
+        /\ B.loc_disjoint (loc p2_buffer) (plaintext2_union p2)
+    )
+    (ensures fun h0 _ h1 ->
+        let p2_s_deserd = plaintext2_eval h1 p2 in
+        let p2_s = Spec.deserialize_ptx2 (as_seq h0 p2_buffer) in
+
+        plaintext2_modifies p2 h0 h1
+        /\ Seq.equal p2_s_deserd.c_R p2_s.c_R
+        /\ Seq.equal p2_s_deserd.id_cred_R p2_s.id_cred_R
+        /\ Seq.equal p2_s_deserd.cred_R p2_s.cred_R
+        /\ Seq.equal p2_s_deserd.mac2 p2_s.mac2
+    )
+
+/// ------------------------
+/// Message 2
+/// ------------------------
+let construct_msg2 (kcs: supportedKemCipherSuite)
+    (ct_y: kem_ciphertext_buff kcs) (ct_auth_I: kem_ciphertext_buff kcs)
+    (c2: c2_buff kcs)
+    : Tot (message2 kcs)
+    = { ct_y = ct_y; ct_auth_I = ct_auth_I; c2 = c2 }
+
+let concat_msg2_get_fixed_length (kcs: supportedKemCipherSuite)
+    = size (SpecCrypto.kem_ciphertext_size kcs) +! size (SpecCrypto.kem_ciphertext_size kcs)
+    +! size (Spec.c2_size kcs)
+
+val concat_msg2:
+    kcs: supportedKemCipherSuite
+    -> msg2: message2 kcs
+    -> msg2_buffer: lbuffer uint8 (concat_msg2_get_fixed_length kcs)
+    -> ST.Stack unit
+    (requires fun h0 ->
+        is_valid_message2 h0 msg2 /\ live h0 msg2_buffer
+        /\ B.loc_disjoint (loc msg2_buffer) (message2_union msg2)
+    )
+    (ensures fun h0 _ h1 ->
+        let m2_s = message2_eval #kcs h0 msg2 in
+        let m2_s_concat = Spec.concat_msg2 #kcs m2_s in
+
+        modifies1 msg2_buffer h0 h1
+        /\ Seq.equal (as_seq h1 msg2_buffer) m2_s_concat
+    )
+
+/// ------------------------
+/// Plaintext 3
+/// ------------------------
+let construct_msg3 (kcs: supportedKemCipherSuite)
+    (id_cred_I: id_cred_buffer) (mac3: mac23_buff kcs)
+    : Tot (plaintext3 kcs)
+    = { id_cred_I = id_cred_I; mac3 = mac3 }
+
+val concat_ptx3:
+    kcs: supportedKemCipherSuite
+    -> p3: plaintext3 kcs
+    -> p3_buffer: plaintext3_buff kcs
+    -> ST.Stack unit
+    (requires fun h0 ->
+        is_valid_plaintext3 h0 p3 /\ live h0 p3_buffer
+        /\ B.loc_disjoint (loc p3_buffer) (plaintext3_union p3)
+    )
+    (ensures fun h0 _ h1 ->
+        let p3_s = plaintext3_eval #kcs h0 p3 in
+        let p3_s_concat = Spec.concat_ptx3 #kcs p3_s in
+
+        modifies1 p3_buffer h0 h1
+        /\ Seq.equal (as_seq h1 p3_buffer) p3_s_concat
+    )
+
+val deserialize_ptx3:
+    kcs: supportedKemCipherSuite
+    -> p3_buffer: plaintext3_buff kcs
+    -> p3: plaintext3 kcs
+    -> ST.Stack unit
+    (requires fun h0 ->
+        is_valid_plaintext3 h0 p3 /\ live h0 p3_buffer
+        /\ B.loc_disjoint (loc p3_buffer) (plaintext3_union p3)
+    )
+    (ensures fun h0 _ h1 ->
+        let p3_s_deserd = plaintext3_eval h1 p3 in
+        let p3_s = Spec.deserialize_ptx3 #kcs (as_seq h0 p3_buffer) in
+
+        plaintext3_modifies p3 h0 h1
+        /\ Seq.equal (as_seq h1 p3.id_cred_I) p3_s.id_cred_I
+        /\ Seq.equal p3_s_deserd.mac3 p3_s.mac3
+    )
